Fix & Prove ex_ocnc

uniana/cfg/CncLoop.v
@@ -7,7 +7,7 @@ Definition cnc_loop `{C : redCFG} h p q
   := loop_contains h p /\ ~ deq_loop q h.
 
 Definition ocnc_loop `{C : redCFG} h p q
-  := cnc_loop h p q /\ forall h', loop_contains h' p -> deq_loop h' h.
+  := cnc_loop h p q /\ forall h', cnc_loop h' p q -> deq_loop h' h.
 
 (*
 (* the ocnc loop has an exit such that q is deeper or equal to the exit *)
@@ -48,9 +48,6 @@ Proof.
       * destruct H3. eapply loop_contains_trans;eauto.
 Qed.
 
-
-
-
 Lemma ex_ocnc_loop `(C : redCFG) p q
       (Hndeq : ~ deq_loop q p)
   : exists h, ocnc_loop h p q .
@@ -61,6 +58,21 @@ Proof.
   destruct Hanc as [[Hp Hq] | Hroot].
   - eapply loop_LPath in Hp as HL.
     destructH.
+
+    (*
+    destr_r' π;subst. 1: inv HL.
+    unfold LPath in HL. path_simpl' HL.
+    destr_r' l;subst.
+    1: {
+      cbn in HL. eapply path_single in HL. destruct HL. subst a.
+      exfalso. eapply Hndeq. eapply loop_contains_deq_loop;eauto.
+    }
+    exists x0.
+    *)
+
+
+
+
     inv_path HL.
     + exfalso.
       eapply Hndeq. eapply loop_contains_deq_loop;eauto.
@@ -69,26 +81,66 @@ Proof.
       copy HL HL'.
       eapply path_rcons_inv' in HL.
       destructH.
-      exists p0. unfold ocnc_loop. split.
-      * unfold cnc_loop. split.
-        -- destruct HL1.
-           destruct l.
-           ++ eapply path_single in HL0. inv HL0.
-              cbn in H. eapply path_single in H. inv H.
-              decide (loop_head p). 1: eapply loop_contains_self;eauto.
-              exfalso.
-              do 2 simpl_dec' Hndeq. destructH. destructH.
-              eapply Hndeq1.
-              eapply H6 in Hndeq0 as QQ. destruct QQ.
-              ** eapply loop_contains_trans;eauto.
-              ** subst x1. exfalso. eapply n. eapply loop_contains_loop_head;eauto.
-           ++ eapply LPath_loop_contains;eauto. congruence.
-        -- destruct HL1. destructH.
-           contradict Hndeq. admit.
-      * intros. admit.
-  - exfalso. subst a. admit.
-Admitted.
+      exists p0. unfold ocnc_loop.
+      assert (loop_contains p0 p) as Hlpp.
+      {
+        destruct HL1.
+        destruct l.
+        - eapply path_single in HL0. inv HL0.
+          cbn in H. eapply path_single in H. inv H.
+          decide (loop_head p). 1: eapply loop_contains_self;eauto.
+          exfalso.
+          do 2 simpl_dec' Hndeq. destructH. destructH.
+          eapply Hndeq1.
+          eapply H6 in Hndeq0 as QQ. destruct QQ.
+          + eapply loop_contains_trans;eauto.
+          + subst x1. exfalso. eapply n. eapply loop_contains_loop_head;eauto.
+        - eapply LPath_loop_contains;eauto. congruence.
+      }
+      split.
+      * unfold cnc_loop.
+        split. 1:eauto.
+        destruct HL1. destructH.
+        contradict Hndeq.
+        specialize (Hnear p0). exploit Hnear.
+        { split;eauto. eapply deq_loop_head_loop_contains;eauto using loop_contains_loop_head. }
+        eapply loop_contains_Antisymmetric in Hnear. exploit Hnear. subst p0. contradiction.
+      * intros. destruct H1.
+        destruct HL1.
+        intros h Hh. destruct H4. eapply H5 in Hh.
+        assert (loop_contains h p) as Hhp.
+        { destruct Hh.
+          - eauto using loop_contains_trans.
+          - subst h. eauto.
+        }
+        eapply loop_contains_either in Hhp as Hpp. 2:eapply H1.
+        destruct Hpp as [Hpp|Hpp]; [|eapply Hpp].
+        destruct Hh.
+        -- contradict H2. eapply loop_contains_deq_loop.
+           eauto using loop_contains_trans.
+        -- subst h.
+           eapply H5 in Hpp. destruct Hpp.
+           ++ contradict H2. eapply loop_contains_deq_loop.
+              eauto using loop_contains_trans.
+           ++ subst h'. eauto using loop_contains_self,loop_contains_loop_head.
+  - subst a.
+    do 2 simpl_dec' Hndeq. destructH.
+    eapply loop_contains_outermost in Hndeq0. destructH.
+    exists h'.
+    split.
+    + destruct Hndeq0.
+      split.
+      * eauto.
+      * intro N. eapply deq_loop_head_loop_contains in N. 2:eauto using loop_contains_loop_head.
+        specialize (Hnear h'). exploit Hnear.
+        eapply root_no_loop;eauto.
+    + intros. destruct H.
+      destruct Hndeq0.
+      eapply loop_contains_deq_loop.
+      eapply H2;eauto.
+Qed.
 
+(* FIXME: this proposition is WRONG *)
 Lemma ocnc_depth `(C : redCFG) h p q
       (Hocnc : ocnc_loop h p q)
   : depth h = S (depth q).
